cedar-lean/Cedar/Thm/PQ.lean
@@ -1,0 +1,88 @@
+/-
+ Copyright Cedar Contributors
+
+ Licensed under the Apache License, Version 2.0 (the "License");
+ you may not use this file except in compliance with the License.
+ You may obtain a copy of the License at
+
+      https://www.apache.org/licenses/LICENSE-2.0
+
+ Unless required by applicable law or agreed to in writing, software
+ distributed under the License is distributed on an "AS IS" BASIS,
+ WITHOUT WARRANTIES OR CONDITIONS OF ANY KIND, either express or implied.
+ See the License for the specific language governing permissions and
+ limitations under the License.
+-/
+
+import Cedar.Thm.PQ.Discretionary
+import Cedar.Thm.PQ.ResourceScan
+
+/-!
+Proves correctness of two implementation of "permission queries", algorithms for
+listing all resources a principal is authorized to perform an action on.
+-/
+
+namespace Cedar.PQ
+
+open Cedar.Spec
+open Cedar.Data
+open Cedar.Thm
+open Cedar.Validation
+
+/--
+The first algorithm scans resources in the entity store, evaluating policies for
+each resource to see if access is permitted. This algorithm applies optimization
+to restrict the sets of policies, entities and candidate resources.  Defined in
+Cedar.PQ.ResourceScan with the main correctness theorem in
+Cedar.Thm.PQ.ResourceScan.
+
+A resource is returned by `scanResourcesForPrincipal` if and only if it exists
+in the entity store, has the requested resource type, and authorization allows
+access to the resource for the requested principal and action.
+-/
+theorem resource_scan_correct (n : Nat) (schema : Schema) (req : ResourcesForPrincipalRequest) (entities : Entities) (policies : Policies) (r : EntityUID) :
+    validateWithLevel policies schema n = .ok () →
+    schema.validateWellFormed = .ok () →
+    validateRequest schema (req.req r) = .ok () →
+    validateEntities schema entities = .ok () →
+    (r ∈ scanResourcesForPrincipal n schema req entities policies ↔
+    (r ∈ entities ∧ r.ty = req.resourceType ∧ (isAuthorized (req.req r) entities policies).decision = .allow))
+:= by
+  intro h₁ h₂ h₃ h₄
+  constructor
+  · intro h_mem
+    have h_req_eq : Request.mk req.principal req.action r req.context = req.req r := by
+      simp only [ResourcesForPrincipalRequest.req]
+    have h_sound := resource_scan_sound n schema req entities policies r h₁ h₂ h₃ h₄ h_mem
+    simp [h_sound]
+  · intro ⟨h₅, h_ty, h_allow⟩
+    exact resource_scan_complete n schema req entities policies r h₁ h₂ h₃ h₄ h₅ h_ty h_allow
+
+/--
+The second algorithm assumes policies are "discretionary" (have particular
+restricted form), and uses this assumption to limit the candidate resources to
+only the resources which appear explicitly authorized in a policy's scope.
+Defined in Cedar.PQ.Discretionary with the main correctness theorem in
+Cedar.Thm.PQ.Discretionary.
+
+Given a discretionary policy set, a resource is returned by
+`discretionaryResourcesForPrincipal` if and only if it has the requested
+resource type and authorization allows access for the resources with the request
+principal and action.
+
+Notably this theorem does not guarantee that the returned resources actually
+exist in the set of entities. This is by design as the query algorithm
+effectively uses the resource scope conditions in the policy store as the set of
+resource entities.
+-/
+theorem discretionary_resource_for_principal_correct :
+  arePoliciesDiscretionary ps = true →
+    (r ∈ discretionaryResourcesForPrincipal pq es ps ↔ (r.ty = pq.resourceType ∧ (isAuthorized (pq.req r) es ps).decision = .allow))
+:= by
+  intro h_discretionary
+  constructor
+  · exact discretionary_resource_for_principal_sound h_discretionary
+  · intro ⟨h_ty, h_auth⟩
+    exact discretionary_resource_for_principal_complete h_discretionary h_ty h_auth
+
+end PQ
