cedar-lean/Cedar/Thm/PQ/Discretionary/DiscretionaryPolicy.lean
@@ -1,0 +1,170 @@
+/-
+ Copyright Cedar Contributors
+
+ Licensed under the Apache License, Version 2.0 (the "License");
+ you may not use this file except in compliance with the License.
+ You may obtain a copy of the License at
+
+      https://www.apache.org/licenses/LICENSE-2.0
+
+ Unless required by applicable law or agreed to in writing, software
+ distributed under the License is distributed on an "AS IS" BASIS,
+ WITHOUT WARRANTIES OR CONDITIONS OF ANY KIND, either express or implied.
+ See the License for the specific language governing permissions and
+ limitations under the License.
+-/
+
+import Cedar.PQ.Discretionary
+import Cedar.Thm.Authorization
+
+/-!
+This file contains theorems describing the shape and behavior of discretionary policies
+-/
+
+namespace Cedar.PQ
+
+open Cedar.Data
+open Cedar.Spec
+open Cedar.Validation
+open Cedar.Thm
+
+inductive DiscretionaryPolicy (policy : Policy) : Prop where
+  | discretionary {p a r: EntityUID}
+    (hp : policy.principalScope.scope.bound = .some p)
+    (ha : policy.actionScope = .actionScope (.eq a))
+    (hr : policy.resourceScope.scope = .eq r)
+    (hc : policy.condition = []) :
+    DiscretionaryPolicy policy
+
+theorem eq_scope_authorizes_principal {policy : Policy} {req : Request} {es : Entities} {p : EntityUID} :
+  satisfied policy req es = true →
+  policy.principalScope.scope = .eq p →
+  req.principal = p
+:= by
+  intro h_satisfied h_scope
+  have h_eval : evaluate policy.toExpr req es = .ok (.prim (.bool true)) := by
+    simpa [satisfied] using h_satisfied
+  have h_principal := and_true_implies_left_true h_eval
+  replace h_scope : policy.3.1 = Scope.eq p := h_scope
+  simpa [h_scope, evaluate, Var.eqEntityUID, apply₂, PrincipalScope.toExpr, Scope.toExpr] using h_principal
+
+theorem mem_scope_authorizes_principal_ancestor {policy : Policy} {req : Request} {es : Entities} {p : EntityUID} :
+  satisfied policy req es = true →
+  policy.principalScope.scope = .mem p →
+  p = req.principal ∨ (es.ancestorsOrEmpty req.principal).contains p
+:= by
+  intro h_satisfied h_scope
+  have h_eval : evaluate policy.toExpr req es = .ok (.prim (.bool true)) := by
+    simpa [satisfied] using h_satisfied
+  replace h_eval := and_true_implies_left_true h_eval
+  replace h_scope : policy.3.1 = Scope.mem p := h_scope
+  simp only [PrincipalScope.toExpr, Scope.toExpr, h_scope, evaluate, Var.inEntityUID, apply₂, inₑ] at h_eval
+  cases h_eq : (req.principal == p)
+  · right
+    simpa [h_eq] using h_eval
+  · exact .inl $ beq_iff_eq.mp h_eq|>.symm
+
+theorem is_mem_scope_authorizes_principal_ancestor {policy : Policy} {req : Request} {es : Entities} {ty : EntityType} {p : EntityUID} :
+  satisfied policy req es = true →
+  policy.principalScope.scope = .isMem ty p →
+  p = req.principal ∨ (es.ancestorsOrEmpty req.principal).contains p
+:= by
+  intro h_satisfied h_scope
+  have h_eval : evaluate policy.toExpr req es = .ok (.prim (.bool true)) := by
+    simpa [satisfied] using h_satisfied
+  replace h_eval := and_true_implies_left_true h_eval
+  replace h_scope : policy.3.1 = Scope.isMem ty p := h_scope
+  simp only [PrincipalScope.toExpr, Scope.toExpr, h_scope] at h_eval
+  replace h_eval := and_true_implies_right_true h_eval
+  simp only [evaluate, Var.inEntityUID, apply₂, inₑ] at h_eval
+  cases h_eq : (req.principal == p)
+  · right
+    simpa [h_eq] using h_eval
+  · exact .inl $ beq_iff_eq.mp h_eq|>.symm
+
+theorem bound_authorizes_principal_ancestor {policy : Policy} {req : Request} {es : Entities} {p : EntityUID} :
+  satisfied policy req es = true →
+  policy.principalScope.scope.bound = .some p →
+  p = req.principal ∨ (es.ancestorsOrEmpty req.principal).contains p
+:= by
+  intro h_satisfied h_bound
+  cases h_scope : policy.principalScope.scope
+  case any | is =>
+    simp only [Scope.bound, h_scope, reduceCtorEq] at h_bound
+  all_goals
+    simp [Scope.bound, h_scope] at h_bound
+    subst h_bound
+  · simp [eq_scope_authorizes_principal h_satisfied h_scope]
+  · simp [mem_scope_authorizes_principal_ancestor h_satisfied h_scope]
+  · simp [is_mem_scope_authorizes_principal_ancestor h_satisfied h_scope]
+
+theorem eq_action_authorizes_action {policy : Policy} {req : Request} {es : Entities} {a : EntityUID} :
+  satisfied policy req es = true →
+  policy.actionScope = .actionScope (.eq a) →
+  req.action = a
+:= by
+  intro h_satisfied h_scope
+  have h_eval : evaluate policy.toExpr req es = .ok (.prim (.bool true)) := by
+    simpa [satisfied] using h_satisfied
+  replace h_action := and_true_implies_left_true (and_true_implies_right_true h_eval)
+  simpa [h_scope, evaluate, Var.eqEntityUID, apply₂, ActionScope.toExpr, Scope.toExpr] using h_action
+
+theorem eq_resource_authorizes_resource {policy : Policy} {req : Request} {es : Entities} {r : EntityUID} :
+  satisfied policy req es = true →
+  policy.resourceScope.scope = .eq r →
+  req.resource = r
+:= by
+  intro h_satisfied h_scope
+  have h_eval : evaluate policy.toExpr req es = .ok (.prim (.bool true)) := by
+    simpa [satisfied] using h_satisfied
+  replace h_eval := and_true_implies_left_true ∘ and_true_implies_right_true ∘ and_true_implies_right_true $ h_eval
+  replace h_scope : policy.5.1 = Scope.eq r := h_scope
+  simpa [ResourceScope.toExpr, Scope.toExpr, h_scope, evaluate, Var.eqEntityUID, apply₂] using h_eval
+
+theorem discretionary_policy_has_expected_shape {policy : Policy} :
+  isPolicyDiscretionary policy = true → DiscretionaryPolicy policy
+:= by
+  intro h_discretionary
+  simp only [isPolicyDiscretionary, List.beq_nil_eq, Bool.and_eq_true, List.isEmpty_iff] at h_discretionary
+  have ⟨⟨⟨h_principal_ok, h_action_ok⟩, h_resource_ok⟩, h_condition_empty⟩ := h_discretionary
+  have ⟨_, h_p⟩  : ∃ b, policy.principalScope.scope.bound = .some b := by
+    cases h_p : policy.principalScope.scope <;>
+      simp only [h_p, Bool.false_eq_true] at h_principal_ok
+    all_goals
+      simp [Scope.bound]
+  have ⟨_, h_a⟩ : ∃ a, policy.actionScope = ActionScope.actionScope (Scope.eq a) := by
+    cases h_a : policy.actionScope <;>
+      simp only [h_a, Bool.false_eq_true] at h_action_ok
+    rename_i a_scope
+    cases a_scope <;>
+      simp only [Bool.false_eq_true] at h_action_ok
+    simp
+  cases h_r : policy.resourceScope.scope <;>
+    simp only [h_r, Bool.false_eq_true] at h_resource_ok
+  exact DiscretionaryPolicy.discretionary h_p h_a h_r h_condition_empty
+
+theorem discretionary_policy_structure_from_satisfaction {policy : Policy} {req : Request} {es : Entities} :
+  isPolicyDiscretionary policy = true →
+  satisfied policy req es = true →
+  (∃ b, policy.principalScope.scope.bound = .some b ∧
+    (b = req.principal ∨ (es.ancestorsOrEmpty req.principal).contains b)) ∧
+  policy.actionScope = .actionScope (.eq req.action) ∧
+  policy.resourceScope.scope = .eq req.resource ∧
+  policy.condition = []
+:= by
+  intro h_discretionary h_satisfied
+
+  have ⟨h_principal_bound, h_action_bound, h_resource_bound, h_condition⟩ :=
+    discretionary_policy_has_expected_shape h_discretionary
+  have h_principal_match : _ = req.principal ∨ (es.ancestorsOrEmpty req.principal).contains _ :=
+    bound_authorizes_principal_ancestor h_satisfied h_principal_bound
+  have h_action_match : req.action = _ :=
+    eq_action_authorizes_action h_satisfied h_action_bound
+  have h_resource_match : req.resource = _ :=
+    eq_resource_authorizes_resource h_satisfied h_resource_bound
+
+  and_intros
+  · simp [h_principal_bound, h_principal_match]
+  · rw [h_action_bound, h_action_match]
+  · rw [h_resource_bound, h_resource_match]
+  · exact h_condition
