cedar-lean/Cedar/Thm/PQ/ResourceScan/ResourceCandidates.lean
@@ -1,0 +1,166 @@
+/-
+ Copyright Cedar Contributors
+
+ Licensed under the Apache License, Version 2.0 (the "License");
+ you may not use this file except in compliance with the License.
+ You may obtain a copy of the License at
+
+      https://www.apache.org/licenses/LICENSE-2.0
+
+ Unless required by applicable law or agreed to in writing, software
+ distributed under the License is distributed on an "AS IS" BASIS,
+ WITHOUT WARRANTIES OR CONDITIONS OF ANY KIND, either express or implied.
+ See the License for the specific language governing permissions and
+ limitations under the License.
+-/
+import Cedar.Data
+import Cedar.Thm.Authorization
+
+import Cedar.PQ.ResourceScan.ResourceCandidates
+
+namespace Cedar.PQ
+
+open Cedar.Data
+open Cedar.Spec
+open Cedar.Thm
+open Cedar.Validation
+
+theorem not_descendant_implies_not_ancestor {es : Entities} :
+  ¬ (es.descendantsOrEmpty e₀).contains e₁ →
+  ¬ (es.ancestorsOrEmpty e₁).contains e₀
+:= by
+  simp only [Entities.descendantsOrEmpty, Entities.ancestorsOrEmpty]
+  intro h
+  cases he₁ : es.find? e₁ <;> simp
+  · simp [Set.empty, Set.contains, Set.elts]
+  · rename_i ed
+    suffices h₁ : ¬e₀ ∈ ed.ancestors from by
+      simpa [Set.contains] using h₁
+    replace h : ∀ ed, (e₁, ed) ∈ es.kvs → e₀ ∉ ed.ancestors := by
+      simpa [Set.contains, Set.elts] using h
+    exact h ed (Map.find?_mem_toList he₁)
+
+theorem descendant_implies_ancestor {es : Entities} :
+  es.WellFormed →
+  (es.descendantsOrEmpty e₀).contains e₁ →
+  (es.ancestorsOrEmpty e₁).contains e₀
+:= by
+  intro hwf
+  simp only [Entities.descendantsOrEmpty, Entities.ancestorsOrEmpty]
+  cases he₁ : es.find? e₁ <;> simp
+  · replace he₁ := Map.find?_none_all_absent he₁
+    simp [Set.empty, Set.contains, Set.elts, he₁]
+  · rename_i ed
+    suffices h :  ∀ ed', (e₁, ed') ∈ es.kvs → e₀ ∈ ed'.ancestors → e₀ ∈ ed.ancestors from by
+      simpa [Set.contains, Set.elts] using h
+    intro ed' he₁'
+    have hed : ed' = ed := by
+      replace he₁' := Map.mem_toList_find? hwf he₁'
+      simpa [he₁'] using he₁
+    rw [←hed]
+    exact id
+
+theorem descendant_eq_ancestor {es : Entities} :
+  es.WellFormed →
+  (es.descendantsOrEmpty e₀).contains e₁ = (es.ancestorsOrEmpty e₁).contains e₀
+:= by
+  intro hwf
+  cases h₁ : (es.descendantsOrEmpty e₀).contains e₁
+  · have h₂ := @not_descendant_implies_not_ancestor e₀ e₁ es
+    simp only [Bool.not_eq_true] at h₂
+    exact (h₂ h₁).symm
+  · exact (descendant_implies_ancestor hwf h₁).symm
+
+theorem resource_candidates_for_policy_complete {p : Policy}
+  (hc : resource_candidates_for_policy p es = some candidates)
+  (hr : req.resource ∉ candidates)
+  (hp : p.effect = .permit) :
+  evaluate p.toExpr req es = .ok false
+:= by
+  suffices hr_false : evaluate p.resourceScope.toExpr req es = .ok false from
+    resource_scope_false_then_policy_false hr_false
+  simp only [resource_candidates_for_policy, hp] at hc
+  split at hc <;> try contradiction
+  all_goals
+    simp only [Option.some.injEq] at hc
+    rw [←hc] at hr ; clear hc
+    rename_i euid hs
+    have hneq : req.resource ≠ euid := by
+      intro heq
+      simp [heq] at hr
+    simp only [ResourceScope.scope] at hs
+    simp only [ResourceScope.toExpr, Scope.toExpr, hs]
+  · simp [Var.eqEntityUID, evaluate, apply₂, hneq]
+  · rename_i ty
+    have hnin : ¬ (es.descendantsOrEmpty euid).contains req.resource := by
+      rw [Bool.not_eq_true, Set.not_contains_prop_bool_equiv]
+      simp only [List.mem_cons, not_or] at hr
+      exact hr.right
+    replace hnin := not_descendant_implies_not_ancestor hnin
+    cases his : ty == req.resource.ty <;>
+      simp [Var.inEntityUID, Var.isEntityType, Result.as, Coe.coe, Value.asBool, evaluate, apply₁, apply₂, inₑ,  his, hnin, hneq]
+  · have hnin : ¬ (es.descendantsOrEmpty euid).contains req.resource := by
+      rw [Bool.not_eq_true, Set.not_contains_prop_bool_equiv]
+      simp only [List.mem_cons, not_or] at hr
+      exact hr.right
+    replace hnin := not_descendant_implies_not_ancestor hnin
+    simp [Var.inEntityUID, evaluate, apply₂, inₑ, hnin, hneq]
+
+theorem resource_candidates_policies_complete
+  (hc : resource_candidates_for_policies ps es = some rs)
+  (hr : req.resource ∉ rs) :
+  (isAuthorized req es ps).decision = .deny
+:= by
+  suffices h_not_permitted : ¬ IsExplicitlyPermitted req es ps from
+    default_deny _ _ _ h_not_permitted
+
+  simp only [resource_candidates_for_policies, Option.map_eq_some_iff] at hc
+  replace ⟨ _, hc, _ ⟩ := hc
+  subst rs
+
+  simp only [IsExplicitlyPermitted, HasSatisfiedEffect, not_exists, not_and]
+  intro p hp he
+
+  have ⟨ p_candidates, hc₁, hc₂ ⟩ := List.mapM_some_implies_all_some hc p hp
+  simp only [List.mem_flatten, not_exists, not_and] at hr
+
+  have h_false := resource_candidates_for_policy_complete hc₂ (hr p_candidates hc₁) he
+  simp [satisfied, h_false]
+
+theorem resource_candidates_complete'
+  (hr : resource ∉ resource_candidates pq ps es)
+  (he : resource ∈ es)
+  (hty : resource.ty = pq.resourceType) :
+  (isAuthorized (pq.req resource) es ps).decision = .deny
+:= by
+  simp only [resource_candidates, Set.mem_filter] at hr
+  cases hr₁ : resource_candidates_for_policies ps es <;> simp only [hr₁] at hr
+  case some rs =>
+    suffices hr₂ : resource ∉ rs from by
+      apply resource_candidates_policies_complete hr₁
+      simp only [ResourcesForPrincipalRequest.req]
+      exact hr₂
+    replace hr : resource ∈ Map.keys es → resource ∉ rs := by
+      simpa [hty] using hr
+    exact hr he
+  case none =>
+    replace hr : resource.ty ≠ pq.resourceType := by
+      simpa [he, Map.in_keys_iff_in_map] using hr
+    simp [hr] at hty
+
+theorem resource_candidates_complete : ∀ {pq ps es resource},
+    resource.ty = pq.resourceType →
+    resource ∈ es →
+    (isAuthorized (pq.req resource) es ps).decision = .allow  →
+    resource ∈ resource_candidates pq ps es := by
+  intro pq es ps r h₁ h₂ h₃
+  have h₄ := mt (@resource_candidates_complete' pq es ps r)
+  simp only [not_imp, Classical.not_not, and_imp] at h₄
+  apply h₄ h₂ h₁
+  simp [h₃]
+
+theorem resource_candidates_sound : ∀ {pq ps es resource},
+    resource ∈ resource_candidates pq ps es → (resource.ty = pq.resourceType ∧ resource ∈ es) := by
+  intro pq ps es r hr
+  simp only [resource_candidates, Set.mem_filter, Bool.and_eq_true, beq_iff_eq] at hr
+  exact .intro hr.right.left hr.left
